src/3d/prelude/buffer/EverParse3d.Actions.All.fsti
@@ -3,10 +3,10 @@ include EverParse3d.Actions.Base
 
 inline_for_extraction
 noextract
-val __PUINT8: Type0
+val ___PUINT8: Type0
 
 noextract
 inline_for_extraction
 val action_field_ptr
       (#nz:_) (#wk: _) (#k:Prelude.parser_kind nz wk) (#t:Type) (#p:Prelude.parser k t) (u:unit)
-   : action p true_inv eloc_none true __PUINT8
+   : action p true_inv eloc_none true ___PUINT8
